Added more features.

Isabelle2/AbstractMultiPaxosWithRecovery2.thy
@@ -2,6 +2,8 @@ theory AbstractMultiPaxosWithRecovery2
   imports Utils MaxByKey IOA Quorums Paxos_Sig "~~/src/HOL/Library/Monad_Syntax"
 begin
 
+text {* TODO: add rejoin; add log truncation *}
+
 section {* Local state and transitions *}
 
 subsection {* Data structures *}
@@ -11,7 +13,7 @@ record ('a, 'v) acc =
   id :: 'a
   acceptors :: "'a set"
   ballot :: bal
-  decision :: "inst \<rightharpoonup> 'v"
+  log :: "inst \<rightharpoonup> 'v"
     -- {* Last ballot in which the acceptor voted. *}
   inst_status :: "bal \<rightharpoonup> (inst \<rightharpoonup> 'v)"
     -- {* After leadership is acquired in ballot b, this describes the result of the 
@@ -19,13 +21,15 @@ record ('a, 'v) acc =
   votes :: "inst \<rightharpoonup> ('v \<times> bal)"
     -- {* The last vote in each instance. *}
   onebs :: "bal \<Rightarrow> ('a \<rightharpoonup> (inst \<times> (inst \<rightharpoonup> ('v\<times>bal))))"
-    -- {* The oneb messages received when the acceptor tries to acquire leadership.
-    Note that we need the outermost option to signify that we did not receive a oneb message
+    -- {* The oneb messages rcvd when the acceptor tries to acquire leadership.
+    Note that we need the outermost option to signify that we did not rcv a oneb message
     from the acceptor, as opposed to receiving a oneb message from an acceptor that never voted. *}
   twobs :: "bal \<Rightarrow> inst \<Rightarrow> 'a set"
-    -- {* the twob messages received (they are broadcast). *}
+    -- {* the twob messages rcvd (they are broadcast). *}
   decisions :: "inst \<Rightarrow> 'a \<rightharpoonup> 'v"
     -- {* Decisions by other processes known to the current process. *}
+  rejoin_resps :: "'a \<rightharpoonup> inst option"
+  restarting :: "bool"
   lowest :: "inst"
   bound :: "inst"
 
@@ -36,6 +40,8 @@ datatype ('a,'v) msg =
   | Phase2b 'a bal inst 'v
   | Fwd 'v
   | Decision 'a inst 'v
+  | ReJoin 'a
+  | ReJoinResp 'a "inst option"
   
 datatype ('a,'v) packet =
   Packet 'a  "('a,'v) msg"
@@ -49,9 +55,10 @@ locale amp_r3 =
 begin
 
 definition local_start where "local_start a \<equiv>
-  \<lparr>id = a, acceptors = as, ballot = 0, decision =\<lambda> i . None, inst_status = \<lambda> i . None,
+  \<lparr>id = a, acceptors = as, ballot = 0, log =\<lambda> i . None, inst_status = \<lambda> i . None,
   votes = \<lambda> i . None, onebs = \<lambda> b a . None,
-  twobs = \<lambda> b i . {}, decisions = \<lambda> i a . None, lowest = 0, bound = lookahead\<rparr>"
+  twobs = \<lambda> b i . {}, decisions = \<lambda> i a . None, rejoin_resps = \<lambda> a . None, 
+  restarting = False, lowest = 0, bound = lookahead\<rparr>"
   
 end
 
@@ -67,12 +74,12 @@ definition next_inst where "next_inst s \<equiv>
   SOME i . inst_status s i = None"
 
 definition do_2a where "do_2a s v \<equiv>
-  let i = next_inst s in if (i \<le> bound s) then
+  let i = next_inst s in if (\<not> restarting s \<and> i \<le> bound s) then
     (let b = ballot s;
       s' = s\<lparr>inst_status := (inst_status s)(b := map_option (\<lambda> f . f(i := Some v)) (inst_status s b)),
         twobs := (twobs s)(b := (twobs s b)(i := {id s}))\<rparr>;
       msgs = send_all s (Phase2a b i v)
-    in (s', msgs)) 
+    in (s', msgs))
   else (s, {})"
  
 definition propose where "propose s v \<equiv>
@@ -81,9 +88,9 @@ definition propose where "propose s v \<equiv>
     then (do_2a s v)
     else (s, {Packet l (Fwd v)})"
 
-subsection {* The @{text receive_fwd} action *}
+subsection {* The @{text rcv_fwd} action *}
 
-definition receive_fwd where "receive_fwd s v \<equiv>
+definition rcv_fwd where "rcv_fwd s v \<equiv>
   let l = leader (ballot s) in
     if l = id s
     then do_2a s v
@@ -102,12 +109,12 @@ definition try_acquire_leadership where "try_acquire_leadership s \<equiv>
     s' = s\<lparr>onebs := (onebs s)(b := ((onebs s b)(a := Some (lowest s, votes s)))), 
       ballot := b\<rparr>;
     msgs = send_all s (Phase1a b)
-  in (s', msgs)"
+  in if \<not> restarting s then (s', msgs) else (s, {})"
 
-subsection {* The @{text receive_1a} action *}
+subsection {* The @{text rcv_1a} action *}
 
-definition receive_1a where "receive_1a s b \<equiv>
-  if b > ballot s then let
+definition rcv_1a where "rcv_1a s b \<equiv>
+  if \<not> restarting s \<and> b > ballot s then let
       msgs = {Packet (leader b) (Phase1b (id s) b (lowest s) (votes s))};
       s' = s\<lparr>ballot := b\<rparr>
     in (s', msgs)
@@ -115,7 +122,7 @@ definition receive_1a where "receive_1a s b \<equiv>
   
 end
 
-subsection {* The @{text receive_1b} action *}
+subsection {* The @{text rcv_1b} action *}
 
 context amp_r3 begin
 
@@ -126,30 +133,31 @@ definition status_from_1bs where
     let votes = {x . \<exists> a \<in> accs . \<exists> f l . bs a = Some (l, f) \<and> f i = Some x \<and> l \<ge> i}
     in (if votes = {} then None else Some (fst (the_elem (max_by_key votes snd))))"
 
-definition msgs_2a where "msgs_2a l bnd bs accs log b \<equiv>
+definition msgs_2a where "msgs_2a low bnd bs accs lg b \<equiv>
   let to_complete = (\<lambda> i . 
-    if (l \<le> i \<and> i \<le> bnd) 
-    then (case log i of Some v \<Rightarrow> None | None \<Rightarrow> (status_from_1bs bs accs i))
+    if (low \<le> i \<and> i \<le> bnd) 
+    then (case lg i of Some v \<Rightarrow> None | None \<Rightarrow> (status_from_1bs bs accs i))
     else None)
   in {Phase2a b i v | i v . to_complete i = Some v}"
 
-definition receive_1b where "receive_1b s a b l vs \<equiv>
+definition rcv_1b where "rcv_1b s a b l vs \<equiv> if \<not> restarting s then (
   let s' = s\<lparr>onebs := (onebs s)(b := ((onebs s b)(a := Some (l, vs))))\<rparr>
   in (if (inst_status s b = None \<and> (\<forall> a \<in> acceptors s . onebs s' b a \<noteq> None))
     then let
         s'' = s'\<lparr>inst_status := (inst_status s)(b := Some (status_from_1bs (onebs s b) (acceptors s)))\<rparr>;
-        msgs = msgs_2a (lowest s) (bound s) (onebs s b) (acceptors s) (decision s) b;
+        msgs = msgs_2a (lowest s) (bound s) (onebs s b) (acceptors s) (log s) b;
         pcks = \<Union> {send_all s m | m . m \<in> msgs}
       in (s'', pcks)
-    else (s', {}))"
+    else (s', {}))) 
+    else (s, {})"
 
-subsection {* The @{text receive_2a} action *}
+subsection {* The @{text rcv_2a} action *}
 
 abbreviation (input) decided where "decided s i \<equiv> 
-  case (decision s i) of Some _ \<Rightarrow> True | _ \<Rightarrow> False"
+  case (log s i) of Some _ \<Rightarrow> True | _ \<Rightarrow> False"
   
-definition receive_2a where "receive_2a s i b v \<equiv>
-  if b \<ge> ballot s \<and> i \<ge> lowest s then
+definition rcv_2a where "rcv_2a s b i v \<equiv>
+  if \<not> restarting s \<and> b \<ge> ballot s \<and> i \<ge> lowest s then
     let s' = s\<lparr>votes := (votes s)(i := Some (v, b)),
       twobs := (twobs s)(b := (twobs s b)(i := insert (id s) (twobs s b i))),
       ballot := b\<rparr>;
@@ -157,34 +165,64 @@ definition receive_2a where "receive_2a s i b v \<equiv>
     in (s', msgs)
   else (s, {})"
   
-subsection {* The @{text receive_2b} action *}
+subsection {* The @{text rcv_2b} action *}
 
-definition receive_2b where "receive_2b s i b a v \<equiv>
-  if (~ decided s i) \<and> i \<ge> lowest s
+definition rcv_2b where "rcv_2b s i b a v \<equiv>
+  if \<not> restarting s \<and> (~ decided s i) \<and> i \<ge> lowest s
   then let
       s' = s\<lparr>twobs := (twobs s)(i := (twobs s i)(b := insert a (twobs s i b)))\<rparr>
     in (
       if (twobs s' i b = (acceptors s))
-      then let s'' = s'\<lparr>decision := (decision s)(i := Some v)\<rparr>
+      then let s'' = s'\<lparr>log := (log s)(i := Some v)\<rparr>
         in (s'', send_all s (Decision (id s) i v))
       else (s', {}) )
   else (s, {})"
-  
-definition receive_decision where "receive_decision s a i v \<equiv>
-  let s' = s\<lparr>decision := (decision s)(i := Some v), decisions := (decisions s)(i := (
+   
+subsection {* The @{text rcv_decision} action *}
+ 
+definition rcv_decision where "rcv_decision s a i v \<equiv>
+  let s' = s\<lparr>log := (log s)(i := Some v), decisions := (decisions s)(i := (
     decisions s i)(a := Some v))\<rparr>;
     s'' = if (\<forall> a \<in> acceptors s . decisions s i a \<noteq> None \<and> i < bound s) then s'\<lparr>bound := i\<rparr> else s'
   in (s', {})"
 
+subsection {* The @{text restart} action *}
+
+definition restart where "restart s \<equiv>
+  (local_start (id s)\<lparr>restarting := True\<rparr>, send_all s (ReJoin (id s)))"
+  
+subsection {* The @{text rcv_rejoin} action *}
+
+definition rcv_rejoin where "rcv_rejoin s src \<equiv>
+    let 
+      ds = {i . log s i \<noteq> None};
+      resp = if ds = {} then None else Some (Max ds)
+    in
+  (s, {Packet src (ReJoinResp (id s) resp)})"
+
+subsection {* The @{text rcv_rejoin_resp} action *}
+  
+definition rcv_rejoin_resp where "rcv_rejoin_resp s a io \<equiv> if restarting s then (
+  let s' = s\<lparr>rejoin_resps := (rejoin_resps s)(a := Some io)\<rparr>
+  in if \<forall> a . rejoin_resps s a \<noteq> None
+    then let 
+        rs = {i . \<exists> a . rejoin_resps s a = Some (Some i)};
+        l = if rs = {} then lookahead+1 else (Max rs)+lookahead+2
+      in (s'\<lparr>lowest := l, restarting := False\<rparr>, {})
+    else (s', {}) )
+  else (s, {})"
+
 subsection {* The @{text process_msg} action *}
 
 fun process_msg where
-  "process_msg s (Phase1a b) = receive_1a s b"
-  | "process_msg s (Phase2a b i v) = receive_2a s i b v"
-  | "process_msg s (Phase1b a b i vs) = receive_1b s a b i vs"
-  | "process_msg s (Phase2b a i b v) = receive_2b s i b a v"
-  | "process_msg s (Fwd v) = receive_fwd s v"
-  | "process_msg s (Decision a i v) = receive_fwd s v"
+  "process_msg s (Phase1a b) = rcv_1a s b"
+  | "process_msg s (Phase2a b i v) = rcv_2a s b i v"
+  | "process_msg s (Phase1b a b i vs) = rcv_1b s a b i vs"
+  | "process_msg s (Phase2b a i b v) = rcv_2b s i b a v"
+  | "process_msg s (Fwd v) = rcv_fwd s v"
+  | "process_msg s (Decision a i v) = rcv_decision s a i v"
+  | "process_msg s (ReJoin a) = rcv_rejoin s a"
+  | "process_msg s (ReJoinResp a io) = rcv_rejoin_resp s a io"
 
 end
 
@@ -199,74 +237,93 @@ context amp_r3 begin
 definition global_start where "global_start \<equiv>
   \<lparr>lstate = (\<lambda> a . local_start a), network = {}\<rparr>"
 
-inductive trans_rel :: "(('a,'v) global_state \<times> 'v paxos_action \<times> ('a,'v) global_state) \<Rightarrow> bool" where
+inductive trans_rel :: "(('a,'v) global_state \<times> ('a,'v) paxos_action \<times> ('a,'v) global_state) \<Rightarrow> bool" where
   "\<lbrakk>(Packet a m) \<in> network s; process_msg ((lstate s) a) m = (sa', ms); m = Phase2b a i b v;
-    decision ((lstate s) a) \<noteq> decision sa'\<rbrakk>
-    \<Longrightarrow> trans_rel (s, Learn i v, 
+    log ((lstate s) a) \<noteq> log sa'\<rbrakk>
+    \<Longrightarrow> trans_rel (s, Learn a i [v],
       s\<lparr>lstate := (lstate s)(a := sa'), network := network s \<union> ms\<rparr>)"
 | "\<lbrakk>(Packet a m) \<in> network s; process_msg ((lstate s) a) m = (sa', ms)\<rbrakk>
     \<Longrightarrow> trans_rel (s, Internal, 
-      s\<lparr>lstate := (lstate s)(a := sa'), network := network s \<union> ms\<rparr>)"
+      s\<lparr>lstate := (lstate s)(a := sa'), network := network s \<union> ms\<rparr>)" 
 | "\<lbrakk>propose ((lstate s) a) v = (sa', ms)\<rbrakk>
     \<Longrightarrow> trans_rel (s, Propose v, 
       s\<lparr>lstate := (lstate s)(a := sa'), network := network s \<union> ms\<rparr>)"
 | "\<lbrakk>try_acquire_leadership ((lstate s) a) = (sa', ms)\<rbrakk>
     \<Longrightarrow> trans_rel (s, Internal, 
       s\<lparr>lstate := (lstate s)(a := sa'), network := network s \<union> ms\<rparr>)"
+| "\<lbrakk>restart ((lstate s) a) = (sa', ms)\<rbrakk>
+    \<Longrightarrow> trans_rel (s, Internal, 
+      s\<lparr>lstate := (lstate s)(a := sa'), network := network s \<union> ms\<rparr>)"
   
 inductive_cases trans_rel_cases:"trans_rel (s,a,s')"
 
-abbreviation(input) local_step where "local_step a p r r' \<equiv> 
+abbreviation (input) local_step where "local_step a p r r' \<equiv> 
   r' = r\<lparr>lstate := (lstate r)(a := fst p), network := network r \<union> snd p\<rparr>"
   
 lemma trans_cases:
   assumes "trans_rel (r, act, r')"
   obtains
     (propose) a v where "act = Propose v" and "local_step a (propose (lstate r a) v) r r'"
-  | (learn) a i b v m p where "act = Learn i v" and "m = Phase2b a i b v"
-    and "p = receive_2b (lstate r a) i b a v"
+  | (learn) a i b v m p where "act = Learn a i [v]" and "m = Phase2b a i b v"
+    and "p = rcv_2b (lstate r a) i b a v"
     and "local_step a p r r'"
     and "Packet a m \<in> network r" 
-    and "decision (lstate r a) \<noteq> decision (fst p)"
+    and "log (lstate r a) \<noteq> log (fst p)"
   | (acquire_leadership) a where "act = Internal" and "local_step a (try_acquire_leadership (lstate r a)) r r'"
-  | (receive_1a) a b m p where "act = Internal" and "m = Phase1a b"
-    and "p = receive_1a (lstate r a) b"
+  | (rcv_1a) a b m p where "act = Internal" and "m = Phase1a b"
+    and "p = rcv_1a (lstate r a) b"
     and "local_step a p r r'"
-    and "Packet a m \<in> network r"
-  | (receive_2a) a i b v m p where "act = Internal" and "m = Phase2a i b v"
-    and "p = receive_2a (lstate r a) i b v"
+    and "Packet a m \<in> network r" 
+  | (rcv_2a) a b i v m p where "act = Internal" and "m = Phase2a b i v"
+    and "p = rcv_2a (lstate r a) b i v"
     and "local_step a p r r'"
-    and "Packet a m \<in> network r"
-  | (receive_2b) a a2 i b v m p where "act = Internal" and "m = Phase2b a2 i b v"
-    and "p = receive_2b (lstate r a) i b a2 v"
+    and "Packet a m \<in> network r" 
+  | (rcv_2b) a a2 i b v m p where "act = Internal" and "m = Phase2b a2 i b v"
+    and "p = rcv_2b (lstate r a) i b a2 v"
     and "local_step a p r r'"
-    and "Packet a m \<in> network r"
-  | (receive_1b) a b vs m p a2 where "act = Internal" and "m = Phase1b a2 b vs"
-    and "p = receive_1b (lstate r a) a2 b vs"
+    and "Packet a m \<in> network r" 
+  | (rcv_1b) a b i vs m p a2 where "act = Internal" and "m = Phase1b a2 b i vs"
+    and "p = rcv_1b (lstate r a) a2 b i vs"
     and "local_step a p r r'"
-    and "Packet a m \<in> network r"
+    and "Packet a m \<in> network r" 
   | (fwd) a v m p where "act = Internal" and "m = Fwd v"
-    and "p = receive_fwd (lstate r a) v"
+    and "p = rcv_fwd (lstate r a) v"
     and "local_step a p r r'"
     and "Packet a m \<in> network r"
+  | (rcv_decision) a a2 i v p m where "act = Internal" and "m = Decision a2 i v"
+    and "p = rcv_decision (lstate r a) a2 i v"
+    and "local_step a p r r'"
+    and "Packet a m \<in> network r"
+  | (rcv_rejoin) a a2 p m where "act = Internal" and "m = ReJoin a2"
+    and "p = rcv_rejoin (lstate r a) a2"
+    and "local_step a p r r'"
+  | (rcv_rejoin_resp) a a2 io p m where "act = Internal" and "m = ReJoinResp a2 io"
+    and "p = rcv_rejoin_resp (lstate r a) a2 io"
+    and "local_step a p r r'"
+  | (restart) a p m where "act = Internal"
+    and "p = restart (lstate r a)"
+    and "local_step a p r r'"
 proof -
   show ?thesis using assms
     apply (rule trans_rel_cases)
-       apply (metis fst_conv learn snd_conv)
-      defer
-      apply (metis fst_conv propose snd_conv)
-     apply (metis acquire_leadership fst_conv snd_conv)
-    subgoal premises prems for a m (* TODO: how to apply induct here without subgoal? *)
-      using prems
-      apply (induct rule:process_msg.induct)
-          apply (metis fst_conv process_msg.simps(1) receive_1a snd_conv)
-         apply (metis fst_conv process_msg.simps(2) receive_2a snd_conv)
-        defer
-        apply (metis fst_conv process_msg.simps(4) receive_1b snd_conv)
-       apply (metis amp_r3.process_msg.simps(5) fst_conv fwd snd_conv)
-      by (metis fst_conv process_msg.simps(3) receive_2b snd_conv)
+    subgoal premises prems using learn prems by (metis fst_conv snd_conv)
+       defer
+    subgoal premises prems using propose prems by (metis fst_conv snd_conv)
+    subgoal premises prems using acquire_leadership prems by (metis fst_conv snd_conv) 
+    subgoal premises prems using restart prems by (metis fst_conv snd_conv)
+    subgoal premises prems for a m s' msgs using prems
+      apply (induct rule:process_msg.induct; simp)
+      subgoal premises prems using rcv_1a prems by (metis fst_conv snd_conv)
+      subgoal premises prems using rcv_2a prems by (metis fst_conv snd_conv)
+      subgoal premises prems using rcv_1b prems  by (metis fst_conv snd_conv) 
+      subgoal premises prems using rcv_2b prems by (metis fst_conv snd_conv)
+      subgoal premises prems using fwd prems by (metis fst_conv snd_conv) 
+      subgoal premises prems using rcv_decision prems  by (metis fst_conv snd_conv) 
+      subgoal premises prems using rcv_rejoin prems by (metis fst_conv snd_conv)
+      subgoal premises prems using rcv_rejoin_resp prems by (metis fst_conv snd_conv)
+      done
     done
-qed
+qed 
 
 definition ioa where
   "ioa \<equiv> \<lparr>ioa.asig = paxos_asig, ioa.start = {global_start}, ioa.trans = Collect trans_rel\<rparr>"
